Demonstre que $\forall x,y, z \in \mathbb{N}, x \cdot (y + z) = (x \cdot y + x \cdot z)$. \\
\emph{Resolução.}\\
Aplicaremos indução sobre $z$. \\
Seja $P(n) := \forall x, y \in \mathbb{N}, x \cdot (y + n) = (x \cdot y + x \cdot n)$. \\
Passo base: $n = 0$
\begin{align*}
	P(0) & = x \cdot (y + 0)                                   \\
	     & = x \cdot y                 & \quad \text{(Por A1)} \\
	     & = (x \cdot y) + 0           & \quad \text{(Por A1)} \\
	     & = (x \cdot y) + (x \cdot 0) & \quad \text{(Por M1)}
\end{align*}
Logo, $P(0)$ é verdadeiro. \\
Passo indutivo: \\
Seja um certo $k \in \mathbb{N}$ tal que
\begin{displaymath}
	\forall x,y \in \mathbb{N}, x \cdot (y + k) = (x \cdot y) + (x \cdot k) \quad \text{(Hipótese Indutiva)}
\end{displaymath}
(Provemos que $P(Suc(k)):= x \cdot (y + Suc(k)) = (x \cdot y) + (x \cdot Suc(k))$) \\
Logo:
\begin{align*}
	P(Suc(k)) & = x \cdot (y + Suc(k))                                   \\
	          & = x \cdot Suc(y + k)             & \quad \text{(Por A2)} \\
	          & = x \cdot (y + k) + x            & \quad \text{(Por M2)} \\
	          & = (x \cdot y) + (x \cdot k) + x  & \quad \text{(Por HI)} \\
	          & = (x \cdot y) + (x \cdot Suc(k)) & \quad \text{(Por M2)} \\
\end{align*}
Portanto, $P(Suc(k))$ é verdadeiro e o teorema é válido.