Demonstre que $\forall n \in \mathbb{N}$:
\begin{displaymath}
	\sum\limits_{i=1}^n i^2 = \frac{n (2n+1) (n+1)}{6}
\end{displaymath}
\emph{Resolução.} 
\begin{enumerate}
	\item Indução sobre $n$.
	\item Seja $\forall n \in \mathbb{N}, P(n) := \sum\limits_{i=1}^n i^2 = \frac{n (2n+1) (n+1)}{6}$.
	\item Passo-base: $P(1)$
	\begin{align*}
		\sum\limits_{i=1}^1 i^2 &= 1^2 &\quad(\text{Por def. rec. de $\sum$}) \\
		&= 1 \\
		&= \frac{6}{6} &\quad(\text{Por arit.}) \\
		&= \frac{1 \cdot (2 \cdot 1 + 1) \cdot (1 + 1)}{6} \\
		&= \frac{n \cdot (2n + 1) \cdot (n + 1)}{6} &\quad \text{(Para $n = 1$)}  
	\end{align*}
	Logo, $P(1)$ é verdadeiro.
	\item Para um certo $k \in \mathbb{N}, P(k):= \sum\limits_{i=1}^k i^2 = \frac{k (2k+1) (k+1)}{6}$ (Hipótese Indutiva). \\
	(Provemos que $P(k+1) = \frac{(k+1) (2 \cdot (k+1) + 1) (k + 2)}{6}$). \\
	\item Então, temos:
	\begin{align*}
		P(k+1) &= \sum\limits_{i=1}^{k+1} i^2 \\
		&= (\sum\limits_{i=1}^{k} i^2) + (k+1)^2 &\quad \text{(Por def. rec. de $\sum$)} \\
		&= \frac{k (2k+1) (k+1)}{6} + (k+1)^2 &\quad \text{(Por HI)}\\
		&= \frac{k (2k+1) (k+1) + 6(k+1)^2}{6} &\quad \text{(Por arit.)}\\
		&= \frac{(2k^2 + k) (k+1) + 6k^2 + 12k + 6}{6} &\quad \text{(Por arit.)}\\
		&= \frac{2k^3 + 3k^2 + k + 6k^2 + 12k + 6}{6} &\quad \text{(Por arit.)}\\
		&= \frac{2k^3 + 9k^2 + 13k + 6}{6} &\quad \text{(Por arit.)}\\
		&= \frac{(k + 1) (2 \cdot (k+1) + 1) (k + 2)}{6} &\quad \text{(Por arit.)}\\
	\end{align*}
	Logo, $P(k+1)$ é verdadeiro e a proposição inicial é verdadeira.
\end{enumerate}
